cedar-lean/Cedar/Thm/Validation/WellTyped/TypeLifting.lean
@@ -154,6 +154,7 @@ theorem lifted_type_is_lifted (ty : CedarType) :
     have := lifted_type_is_lifted ty'
     exact Lifted.set this
   case record rty =>
+    simp only [RecordType.liftBoolTypes]
     unfold CedarType.liftBoolTypesRecord
     split
     case _ heq =>
@@ -304,7 +305,8 @@ theorem lifted_type_is_top {ty₁ ty₂ : CedarType} :
       rcases heq with ⟨_, h₁, h₂⟩
       simp [h] at h₂
       simp [h₂] at h₁
-      simp [CedarType.liftBoolTypes]
+      simp only [CedarType.liftBoolTypes, RecordType.liftBoolTypes, CedarType.record.injEq,
+        Data.Map.mk.injEq]
       exact lifted_record_type_is_top (lubRecordType_is_lub_of_record_types h₁)
     case _ =>
       split at heq
